\section{The Double Orientation Cover}

\textcolor{red}{While we are trying to decide how to focus the paper, I thought for now I would at least write up some of the information that will be in the paper regardless}

Let $M$ be a non-orientable 3-manifold, $\wt{M}$ its double orientation cover (with covering map $p$), and $\iota: \wt{M} \xrightarrow[]{} \wt{M}$ the involution generating the deck group of the cover.

\begin{lem}
Given $\alpha \in H^1(\wt{M})$, let $[\wt{M}] \frown \alpha$ denote its Poincar\'e dual. Then $\iota^*\alpha = \alpha$ if and only if $\iota_*([\wt{M}] \frown \alpha) = -([\wt{M}] \frown \alpha)$ 
\end{lem}
\begin{proof}
Suppose that $\iota^*\alpha = \alpha$, then:
\begin{align*}
    \iota_*([\wt{M}] \frown \alpha) = \iota_*([\wt{M}] \frown \iota^*\alpha) = \iota_*[\wt{M}] \frown \alpha = -[\wt{M}] \frown \alpha = -([\wt{M}] \frown \alpha)
\end{align*}
Where the second-to-last equality is by $\iota$ being orientation reversing and the last equality is from the bilinearity of the cap product.

Now suppose that $\iota_*([\wt{M}] \frown \alpha) = -([\wt{M}] \frown \alpha)$, then:
\begin{align*}
    \iota_*([\wt{M}] \frown \iota^*\alpha) = \iota_*[\wt{M}] \frown \alpha = -[\wt{M}] \frown \alpha = -([\wt{M}] \cap \alpha) = \iota_*([\wt{M}] \frown \alpha)
\end{align*}
Since $\iota$ is a homeomorphism and thus $\iota_*$ and isomorphism, this implies that $[\wt{M}] \frown \iota^*\alpha = [\wt{M}] \frown \alpha$. Yet taking the cap product with $[\wt{M}]$ is exactly the isomorphism given by Poincar\'e Duality, and thus $\iota^*\alpha = \alpha$.
\end{proof}

\begin{lem}
Let $V \coloneqq$ 1-eigenspace of $\iota$, then $H^1(M) \cong V$ by $p^*$
\end{lem}
\begin{proof}
Covering maps induce innjections on cohomology, so we know that $p^*: H^1(M) \xrightarrow[]{} H^1(\wt{M})$ is an injection and thus isomorphic to its image in $H^1(\wt{M})$. We also know that im$(p^*) \subseteq V$ since if $\alpha = p^*\omega$ for $\omega \in H^1(M)$, then $\iota ^*\alpha = \iota^*p^* \omega = p^* \omega$ by $p = p \circ \iota$. Thus we just need to show that every 1-form in $V$ is a pullback of a 1-form on $M$, so im$(p^*) = V$. To see this, let $\alpha \in V$ be a 1-form on $\wt{M}$ such that $\iota^* \alpha = \alpha$.
\end{proof}
